Implemented remove

BinaryTrees.v
@@ -1,7 +1,6 @@
 Require Import PeanoNat.
 Require Import List.
-
-Scheme All for list.
+Import ListNotations.
 
 Inductive tree : Type :=
   node (label : nat) (branches : list tree).
@@ -12,13 +11,16 @@ Fixpoint rm (t : tree) (target : nat) : option tree :=
   match t with
   | node label branches => if label =? target 
                              then None 
-                             else Some (node label (rm_list branches target))
-  end
-with rm_list (l : list tree) (target : nat) : list tree :=
-  match l with
-  | nil => nil
-  | h::t => match rm h target with
-            | None => rm_list t target
-            | Some tree => tree::(rm_list t target)
-            end
+                             else Some (node label ((fix rm_list (l : list tree) (val : nat) : list tree :=
+                                                    match l with
+                                                    | nil => nil
+                                                    | h::t => match rm h target with
+                                                              | None => rm_list t val
+                                                              | Some tree => tree::(rm_list t val)
+                                                               end
+                                                        end) branches target))
   end.
+
+Example test_rm1: rm (node 1 [(node 3 nil);(node 7 nil);(node 9 nil)]) 3 
+  = Some (node 1 [(node 7 nil);(node 9 nil)]).
+Proof. reflexivity. Qed.
